lean/Protocol/Typing/Framing/GEnvFrameLeft.lean
@@ -176,7 +176,7 @@ lemma HasTypeProcPreOut_frame_G_left
       have hUpd := updateG_append_left (G₁:=Gfr) (G₂:=G) (e:=e) (L:=L) hNone
       simpa [hUpd] using
         (HasTypeProcPreOut.send (Ssh:=Ssh) (Sown:=Sown) (G:=Gfr ++ G) hk hG'' hx)
-  | recv_new hk hG hNoSh hNoOwnL =>
+  | recv_new hk hG hNoSh hNoOwnR hNoOwnL =>
       rename_i Sown G k x e p T L
       have hNone := lookupG_none_of_disjoint hDisj hG
       have hG' := lookupG_append_right (G₁:=Gfr) (G₂:=G) (e:=e) hNone
@@ -184,8 +184,8 @@ lemma HasTypeProcPreOut_frame_G_left
         simpa [hG] using hG'
       have hUpd := updateG_append_left (G₁:=Gfr) (G₂:=G) (e:=e) (L:=L) hNone
       simpa [hUpd] using
-        (HasTypeProcPreOut.recv_new (Ssh:=Ssh) (Sown:=Sown) (G:=Gfr ++ G) hk hG'' hNoSh hNoOwnL)
-  | recv_old hk hG hNoSh hOwn =>
+        (HasTypeProcPreOut.recv_new (Ssh:=Ssh) (Sown:=Sown) (G:=Gfr ++ G) hk hG'' hNoSh hNoOwnR hNoOwnL)
+  | recv_old hk hG hNoSh hNoOwnR hOwn =>
       rename_i Sown G k x e p T L T'
       have hNone := lookupG_none_of_disjoint hDisj hG
       have hG' := lookupG_append_right (G₁:=Gfr) (G₂:=G) (e:=e) hNone
@@ -193,7 +193,7 @@ lemma HasTypeProcPreOut_frame_G_left
         simpa [hG] using hG'
       have hUpd := updateG_append_left (G₁:=Gfr) (G₂:=G) (e:=e) (L:=L) hNone
       simpa [hUpd] using
-        (HasTypeProcPreOut.recv_old (Ssh:=Ssh) (Sown:=Sown) (G:=Gfr ++ G) hk hG'' hNoSh hOwn)
+        (HasTypeProcPreOut.recv_old (Ssh:=Ssh) (Sown:=Sown) (G:=Gfr ++ G) hk hG'' hNoSh hNoOwnR hOwn)
   | select hk hG hbs =>
       rename_i Sown G k l e q bs L
       have hNone := lookupG_none_of_disjoint hDisj hG
@@ -278,11 +278,11 @@ lemma HasTypeProcPreOut_frame_G_left
       exact HasTypeProcPreOut_frame_G_left_par (Ssh:=Ssh) (Gfr:=Gfr) (split:=split)
         hSlen hGlen hSfin hGfin hW hΔ hDisjG hDisjS hDisjS_left hDisjS_right hDisjS'
         hDisjW hDisjΔ hS1 hS2 hP' hQ hDisjGfrG1 hDisjGfrG2
-  | assign_new hNoSh hNoOwnL hv =>
+  | assign_new hNoSh hNoOwnR hNoOwnL hv =>
       rename_i Sown G x v T
       have hv' := HasTypeVal_frame_left (G₁:=Gfr) (G₂:=G) hDisj hv
-      exact HasTypeProcPreOut.assign_new hNoSh hNoOwnL hv'
-  | assign_old hNoSh hOwn hv =>
+      exact HasTypeProcPreOut.assign_new hNoSh hNoOwnR hNoOwnL hv'
+  | assign_old hNoSh hNoOwnR hOwn hv =>
       rename_i Sown G x v T T'
       have hv' := HasTypeVal_frame_left (G₁:=Gfr) (G₂:=G) hDisj hv
-      exact HasTypeProcPreOut.assign_old hNoSh hOwn hv'
+      exact HasTypeProcPreOut.assign_old hNoSh hNoOwnR hOwn hv'
